% Generated on 2019-12-09 17:11:54 by gEcon ver. 1.2.0 (2019-09-08)
% http://gecon.r-forge.r-project.org/

% Model name: dsge_model

\section{CONSUMER}

\subsection{Optimisation problem}

\begin{align}
&\max_{C_{t}, H_{t}
} U_{t} = \log{C_{t}} + {\beta} {\mathrm{E}_{t}\left[U_{t+1}\right]} + {\psi} {\log\left(1 - H_{t}\right)}\\
&\mathrm{s.t.:}\nonumber\\
& C_{t} + T_{t} = \Pi_{t} + {H_{t}} {W_{t}} \quad \left(\lambda^{\mathrm{c}}_{t}\right)
\end{align}


\subsection{First order conditions}

\begin{equation}
\beta - \lambda^{\mathrm{U}}_{t} = 0
 \quad \left(U_{t}\right)
\end{equation}
\begin{equation}
-\lambda^{\mathrm{c}}_{t} + {C_{t}}^{-1} = 0
 \quad \left(C_{t}\right)
\end{equation}
\begin{equation}
{\lambda^{\mathrm{c}}_{t}} {W_{t}} - {\psi} \left(1 - H_{t}\right)^{-1} = 0
 \quad \left(H_{t}\right)
\end{equation}




\section{FIRM}

\subsection{Optimisation problem}

\begin{align}
&\max_{K_{t}, H^{\mathrm{d}}_{t}, Y_{t}, I_{t}, \Pi_{t}, {C\!a\!p\!U\!t}_{t}
} {S\!P\!I}_{t} = \Pi_{t} + {\lambda^{\mathrm{c}}_{t}}^{-1} {\mathrm{E}_{t}\left[{\lambda^{\mathrm{U}}_{t+1}} {\lambda^{\mathrm{c}}_{t+1}} {{S\!P\!I}_{t+1}}\right]}\\
&\mathrm{s.t.:}\nonumber\\
& Y_{t} = {{H^{\mathrm{d}}_{t}}^{1 - \alpha}} {\left(e^{Z_{t}}\right)^{1 - \alpha}} {\left({K_{t-1}} {{C\!a\!p\!U\!t}_{t}}\right)^{\alpha}} \quad \left(\lambda^{\mathrm{FIRM}^{\mathrm{1}}}_{t}\right)\\
& K_{t} = I_{t} + {K_{t-1}} \left(1 - {\delta} {{{C\!a\!p\!U\!t}_{t}}^{\omega}}\right) \quad \left(\lambda^{\mathrm{FIRM}^{\mathrm{2}}}_{t}\right)\\
& \Pi_{t} = -I_{t} - {H^{\mathrm{d}}_{t}} {W_{t}} + {P_{t}} {Y_{t}} \quad \left(\lambda^{\mathrm{FIRM}^{\mathrm{3}}}_{t}\right)
\end{align}


\subsection{Identities}

\begin{equation}
K^{\mathrm{ut}}_{t} = {K_{t-1}} {{C\!a\!p\!U\!t}_{t}}
\end{equation}


\subsection{First order conditions}

\begin{equation}
-\lambda^{\mathrm{FIRM}^{\mathrm{SPI}}}_{t} + {\lambda^{\mathrm{c}}_{t-1}}^{-1} {\lambda^{\mathrm{U}}_{t}} {\lambda^{\mathrm{c}}_{t}} = 0
 \quad \left({S\!P\!I}_{t}\right)
\end{equation}
\begin{equation}
-\lambda^{\mathrm{FIRM}^{\mathrm{2}}}_{t} + \mathrm{E}_{t}\left[{\lambda^{\mathrm{FIRM}^{\mathrm{SPI}}}_{t+1}} \left({\lambda^{\mathrm{FIRM}^{\mathrm{2}}}_{t+1}} \left(1 - {\delta} {{{C\!a\!p\!U\!t}_{t+1}}^{\omega}}\right) + {\alpha} {\lambda^{\mathrm{FIRM}^{\mathrm{1}}}_{t+1}} {{C\!a\!p\!U\!t}_{t+1}} {{H^{\mathrm{d}}_{t+1}}^{1 - \alpha}} {\left(e^{Z_{t+1}}\right)^{1 - \alpha}} {\left({K_{t}} {{C\!a\!p\!U\!t}_{t+1}}\right)^{-1 + \alpha}}\right)\right] = 0
 \quad \left(K_{t}\right)
\end{equation}
\begin{equation}
-{\lambda^{\mathrm{FIRM}^{\mathrm{3}}}_{t}} {W_{t}} + {\lambda^{\mathrm{FIRM}^{\mathrm{1}}}_{t}} \left(1 - \alpha\right) {{H^{\mathrm{d}}_{t}}^{-\alpha}} {\left(e^{Z_{t}}\right)^{1 - \alpha}} {\left({K_{t-1}} {{C\!a\!p\!U\!t}_{t}}\right)^{\alpha}} = 0
 \quad \left(H^{\mathrm{d}}_{t}\right)
\end{equation}
\begin{equation}
-\lambda^{\mathrm{FIRM}^{\mathrm{1}}}_{t} + {\lambda^{\mathrm{FIRM}^{\mathrm{3}}}_{t}} {P_{t}} = 0
 \quad \left(Y_{t}\right)
\end{equation}
\begin{equation}
\lambda^{\mathrm{FIRM}^{\mathrm{2}}}_{t} - \lambda^{\mathrm{FIRM}^{\mathrm{3}}}_{t} = 0
 \quad \left(I_{t}\right)
\end{equation}
\begin{equation}
1 - \lambda^{\mathrm{FIRM}^{\mathrm{3}}}_{t} = 0
 \quad \left(\Pi_{t}\right)
\end{equation}
\begin{equation}
-{\delta} {\omega} {K_{t-1}} {\lambda^{\mathrm{FIRM}^{\mathrm{2}}}_{t}} {{{C\!a\!p\!U\!t}_{t}}^{-1 + \omega}} + {\alpha} {K_{t-1}} {\lambda^{\mathrm{FIRM}^{\mathrm{1}}}_{t}} {{H^{\mathrm{d}}_{t}}^{1 - \alpha}} {\left(e^{Z_{t}}\right)^{1 - \alpha}} {\left({K_{t-1}} {{C\!a\!p\!U\!t}_{t}}\right)^{-1 + \alpha}} = 0
 \quad \left({C\!a\!p\!U\!t}_{t}\right)
\end{equation}


\subsection{First order conditions after reduction}

\begin{equation}
-\lambda^{\mathrm{FIRM}^{\mathrm{SPI}}}_{t} + {\lambda^{\mathrm{c}}_{t-1}}^{-1} {\lambda^{\mathrm{U}}_{t}} {\lambda^{\mathrm{c}}_{t}} = 0
 \quad \left({S\!P\!I}_{t}\right)
\end{equation}
\begin{equation}
-1 + \mathrm{E}_{t}\left[{\lambda^{\mathrm{FIRM}^{\mathrm{SPI}}}_{t+1}} \left(1 - {\delta} {{{C\!a\!p\!U\!t}_{t+1}}^{\omega}} + {\alpha} {\lambda^{\mathrm{FIRM}^{\mathrm{1}}}_{t+1}} {{C\!a\!p\!U\!t}_{t+1}} {{H^{\mathrm{d}}_{t+1}}^{1 - \alpha}} {\left(e^{Z_{t+1}}\right)^{1 - \alpha}} {\left({K_{t}} {{C\!a\!p\!U\!t}_{t+1}}\right)^{-1 + \alpha}}\right)\right] = 0
 \quad \left(K_{t}\right)
\end{equation}
\begin{equation}
-W_{t} + {\lambda^{\mathrm{FIRM}^{\mathrm{1}}}_{t}} \left(1 - \alpha\right) {{H^{\mathrm{d}}_{t}}^{-\alpha}} {\left(e^{Z_{t}}\right)^{1 - \alpha}} {\left({K_{t-1}} {{C\!a\!p\!U\!t}_{t}}\right)^{\alpha}} = 0
 \quad \left(H^{\mathrm{d}}_{t}\right)
\end{equation}
\begin{equation}
-\lambda^{\mathrm{FIRM}^{\mathrm{1}}}_{t} + P_{t} = 0
 \quad \left(Y_{t}\right)
\end{equation}
\begin{equation}
-{\delta} {\omega} {K_{t-1}} {{{C\!a\!p\!U\!t}_{t}}^{-1 + \omega}} + {\alpha} {K_{t-1}} {\lambda^{\mathrm{FIRM}^{\mathrm{1}}}_{t}} {{H^{\mathrm{d}}_{t}}^{1 - \alpha}} {\left(e^{Z_{t}}\right)^{1 - \alpha}} {\left({K_{t-1}} {{C\!a\!p\!U\!t}_{t}}\right)^{-1 + \alpha}} = 0
 \quad \left({C\!a\!p\!U\!t}_{t}\right)
\end{equation}




\section{EQUILIBRIUM}

\subsection{Identities}

\begin{equation}
P_{t} = 1
\end{equation}
\begin{equation}
H_{t} = H^{\mathrm{d}}_{t}
\end{equation}




\section{GOVERNMENT}

\subsection{Identities}

\begin{equation}
T_{t} = G_{t}
\end{equation}
\begin{equation}
G_{t} = \epsilon^{\mathrm{G}}_{t} + {\phi^{\mathrm{G}}} {G_{t-1}}
\end{equation}




\section{EXOG}

\subsection{Identities}

\begin{equation}
Z_{t} = \epsilon^{\mathrm{Z}}_{t} + {\phi^{\mathrm{Z}}} {Z_{t-1}}
\end{equation}




\section{Equilibrium relationships (after reduction)}

\begin{equation}
-1 + {\beta} {C_{t}} {\mathrm{E}_{t}\left[{C_{t+1}}^{-1} \left(1 - {\delta} {{{C\!a\!p\!U\!t}_{t+1}}^{\omega}} + {\alpha} {{C\!a\!p\!U\!t}_{t+1}} {{H_{t+1}}^{1 - \alpha}} {\left(e^{Z_{t+1}}\right)^{1 - \alpha}} {\left({K_{t}} {{C\!a\!p\!U\!t}_{t+1}}\right)^{-1 + \alpha}}\right)\right]} = 0
\end{equation}
\begin{equation}
-K^{\mathrm{ut}}_{t} + {K_{t-1}} {{C\!a\!p\!U\!t}_{t}} = 0
\end{equation}
\begin{equation}
-W_{t} + \left(1 - \alpha\right) {{H_{t}}^{-\alpha}} {\left(e^{Z_{t}}\right)^{1 - \alpha}} {\left({K_{t-1}} {{C\!a\!p\!U\!t}_{t}}\right)^{\alpha}} = 0
\end{equation}
\begin{equation}
-Y_{t} + {{H_{t}}^{1 - \alpha}} {\left(e^{Z_{t}}\right)^{1 - \alpha}} {\left({K_{t-1}} {{C\!a\!p\!U\!t}_{t}}\right)^{\alpha}} = 0
\end{equation}
\begin{equation}
{C_{t}}^{-1} {W_{t}} - {\psi} \left(1 - H_{t}\right)^{-1} = 0
\end{equation}
\begin{equation}
-{\delta} {\omega} {K_{t-1}} {{{C\!a\!p\!U\!t}_{t}}^{-1 + \omega}} + {\alpha} {K_{t-1}} {{H_{t}}^{1 - \alpha}} {\left(e^{Z_{t}}\right)^{1 - \alpha}} {\left({K_{t-1}} {{C\!a\!p\!U\!t}_{t}}\right)^{-1 + \alpha}} = 0
\end{equation}
\begin{equation}
\epsilon^{\mathrm{G}}_{t} - G_{t} + {\phi^{\mathrm{G}}} {G_{t-1}} = 0
\end{equation}
\begin{equation}
\epsilon^{\mathrm{Z}}_{t} - Z_{t} + {\phi^{\mathrm{Z}}} {Z_{t-1}} = 0
\end{equation}
\begin{equation}
I_{t} - K_{t} + {K_{t-1}} \left(1 - {\delta} {{{C\!a\!p\!U\!t}_{t}}^{\omega}}\right) = 0
\end{equation}
\begin{equation}
U_{t} - \log{C_{t}} - {\beta} {\mathrm{E}_{t}\left[U_{t+1}\right]} - {\psi} {\log\left(1 - H_{t}\right)} = 0
\end{equation}
\begin{equation}
-C_{t} - G_{t} + {S\!P\!I}_{t} + {H_{t}} {W_{t}} - {\beta} {C_{t}} {\mathrm{E}_{t}\left[{C_{t+1}}^{-1} {{S\!P\!I}_{t+1}}\right]} = 0
\end{equation}
\begin{equation}
-I_{t} - {S\!P\!I}_{t} + Y_{t} - {H_{t}} {W_{t}} + {\beta} {C_{t}} {\mathrm{E}_{t}\left[{C_{t+1}}^{-1} {{S\!P\!I}_{t+1}}\right]} = 0
\end{equation}



\section{Steady state relationships (after reduction)}

\begin{equation}
-1 + {\beta} \left(1 - {\delta} {{{C\!a\!p\!U\!t}_\mathrm{ss}}^{\omega}} + {\alpha} {{C\!a\!p\!U\!t}_\mathrm{ss}} {{H_\mathrm{ss}}^{1 - \alpha}} {\left(e^{Z_\mathrm{ss}}\right)^{1 - \alpha}} {\left({{C\!a\!p\!U\!t}_\mathrm{ss}} {K_\mathrm{ss}}\right)^{-1 + \alpha}}\right) = 0
\end{equation}
\begin{equation}
-K^{\mathrm{ut}}_\mathrm{ss} + {{C\!a\!p\!U\!t}_\mathrm{ss}} {K_\mathrm{ss}} = 0
\end{equation}
\begin{equation}
-W_\mathrm{ss} + \left(1 - \alpha\right) {{H_\mathrm{ss}}^{-\alpha}} {\left(e^{Z_\mathrm{ss}}\right)^{1 - \alpha}} {\left({{C\!a\!p\!U\!t}_\mathrm{ss}} {K_\mathrm{ss}}\right)^{\alpha}} = 0
\end{equation}
\begin{equation}
-Y_\mathrm{ss} + {{H_\mathrm{ss}}^{1 - \alpha}} {\left(e^{Z_\mathrm{ss}}\right)^{1 - \alpha}} {\left({{C\!a\!p\!U\!t}_\mathrm{ss}} {K_\mathrm{ss}}\right)^{\alpha}} = 0
\end{equation}
\begin{equation}
{C_\mathrm{ss}}^{-1} {W_\mathrm{ss}} - {\psi} \left(1 - H_\mathrm{ss}\right)^{-1} = 0
\end{equation}
\begin{equation}
-{\delta} {\omega} {K_\mathrm{ss}} {{{C\!a\!p\!U\!t}_\mathrm{ss}}^{-1 + \omega}} + {\alpha} {K_\mathrm{ss}} {{H_\mathrm{ss}}^{1 - \alpha}} {\left(e^{Z_\mathrm{ss}}\right)^{1 - \alpha}} {\left({{C\!a\!p\!U\!t}_\mathrm{ss}} {K_\mathrm{ss}}\right)^{-1 + \alpha}} = 0
\end{equation}
\begin{equation}
-G_\mathrm{ss} + {\phi^{\mathrm{G}}} {G_\mathrm{ss}} = 0
\end{equation}
\begin{equation}
-Z_\mathrm{ss} + {\phi^{\mathrm{Z}}} {Z_\mathrm{ss}} = 0
\end{equation}
\begin{equation}
I_\mathrm{ss} - K_\mathrm{ss} + {K_\mathrm{ss}} \left(1 - {\delta} {{{C\!a\!p\!U\!t}_\mathrm{ss}}^{\omega}}\right) = 0
\end{equation}
\begin{equation}
U_\mathrm{ss} - \log{C_\mathrm{ss}} - {\beta} {U_\mathrm{ss}} - {\psi} {\log\left(1 - H_\mathrm{ss}\right)} = 0
\end{equation}
\begin{equation}
-C_\mathrm{ss} - G_\mathrm{ss} + {S\!P\!I}_\mathrm{ss} - {\beta} {{S\!P\!I}_\mathrm{ss}} + {H_\mathrm{ss}} {W_\mathrm{ss}} = 0
\end{equation}
\begin{equation}
-I_\mathrm{ss} - {S\!P\!I}_\mathrm{ss} + Y_\mathrm{ss} + {\beta} {{S\!P\!I}_\mathrm{ss}} - {H_\mathrm{ss}} {W_\mathrm{ss}} = 0
\end{equation}






\section{Parameter settings}

\begin{equation}
\alpha = 0.33
\end{equation}
\begin{equation}
\beta = 0.99
\end{equation}
\begin{equation}
\delta = 0.0265
\end{equation}
\begin{equation}
\omega = 1.45
\end{equation}
\begin{equation}
\phi^{\mathrm{G}} = 0.9
\end{equation}
\begin{equation}
\phi^{\mathrm{Z}} = 0.9
\end{equation}
\begin{equation}
\psi = 1.75
\end{equation}


