% Equation 1
\begin{dmath}
\left({C}-\frac{{H}^{{omega}}}{{omega}}\right)^{\left(-{gamma}\right)}={lambda}\, {P}
\end{dmath}
% Equation 2
\begin{dmath}
\left({C}-\frac{{H}^{{omega}}}{{omega}}\right)^{\left(-{gamma}\right)}\, {H}^{{omega}-1}={lambda}\, {W}
\end{dmath}
% Equation 3
\begin{dmath}
{lambdaS}\, \left(1+{i}\right)={lambda}\, \left(1+{rho}\right)
\end{dmath}
% Equation 4
\begin{dmath}
0={sunspot}
\end{dmath}
% Equation 5
\begin{dmath}
{B}=\left(1+{i}\right)\, {B}+{H}\, {W}+{PI}-{T}-{C}\, {P}
\end{dmath}
% Equation 6
\begin{dmath}
{C}=\left(\left(1-{n}\right)^{\frac{1}{{s}}}\, {CD}^{\frac{{s}-1}{{s}}}+{n}^{\frac{1}{{s}}}\, {CF}^{\frac{{s}-1}{{s}}}\right)^{\frac{{s}}{{s}-1}}
\end{dmath}
% Equation 7
\begin{dmath}
{CD}={C}\, \left(1-{n}\right)\, \left(\frac{{PD}}{{P}}\right)^{\left(-{s}\right)}
\end{dmath}
% Equation 8
\begin{dmath}
{CF}={C}\, {n}\, \left(\frac{{PF}}{{P}}\right)^{\left(-{s}\right)}
\end{dmath}
% Equation 9
\begin{dmath}
{P}=\left(\left(1-{n}\right)\, {PD}^{1-{s}}+{n}\, {PF}^{1-{s}}\right)^{\frac{1}{1-{s}}}
\end{dmath}
% Equation 10
\begin{dmath}
{P}\, {G}={T}
\end{dmath}
% Equation 11
\begin{dmath}
\log\left({G}\right)=\left(1-{zetaG}\right)\, \log\left(({G})\right)+\log\left({G}\right)\, {zetaG}+{sG}
\end{dmath}
% Equation 12
\begin{dmath}
{G}=\left(\left(1-{n}\right)^{\frac{1}{{s}}}\, {GD}^{\frac{{s}-1}{{s}}}+{n}^{\frac{1}{{s}}}\, {GF}^{\frac{{s}-1}{{s}}}\right)^{\frac{{s}}{{s}-1}}
\end{dmath}
% Equation 13
\begin{dmath}
{GD}=\left(1-{n}\right)\, \left(\frac{{PD}}{{P}}\right)^{\left(-{s}\right)}\, {G}
\end{dmath}
% Equation 14
\begin{dmath}
{GF}={n}\, \left(\frac{{PF}}{{P}}\right)^{\left(-{s}\right)}\, {G}
\end{dmath}
% Equation 15
\begin{dmath}
{i}=\left(1-{zetai}\right)\, ({i})+{i}\, {zetai}+{kappa}\, \left(\exp\left(\frac{({B})}{({P})\, ({Y})}-\frac{{B}}{{P}\, {Y}}\right)-1\right)+{si}
\end{dmath}
% Equation 16
\begin{dmath}
{AC}=0
\end{dmath}
% Equation 17
\begin{dmath}
{ACD}=\left(1-{n}\right)\, \left(\frac{{PD}}{{P}}\right)^{\left(-{s}\right)}\, {AC}
\end{dmath}
% Equation 18
\begin{dmath}
{ACF}={n}\, \left(\frac{{PF}}{{P}}\right)^{\left(-{s}\right)}\, {AC}
\end{dmath}
% Equation 19
\begin{dmath}
{theta}\, {phi}={MC}-{pD}\, \frac{{sigma}-1}{{sigma}}
\end{dmath}
% Equation 20
\begin{dmath}
\left(1+{rho}\right)\, {theta}=\frac{\frac{1}{{sigma}}\, {pDS}\, {yS}}{{e}}-\frac{\frac{{pDS}\, \frac{{varphi}}{{sigma}}\, \left(\frac{{pDS}}{{pD}}-1\right)}{{pD}}\, {PS}\, {YS}}{{e}}-\left(1-{eta}\right)\, {thetaS}
\end{dmath}
% Equation 21
\begin{dmath}
0={sunspot2}
\end{dmath}
% Equation 22
\begin{dmath}
0={sunspot3}
\end{dmath}
% Equation 23
\begin{dmath}
0={sunspot4}
\end{dmath}
% Equation 24
\begin{dmath}
0={sunspot5}
\end{dmath}
% Equation 25
\begin{dmath}
0={sunspot6}
\end{dmath}
% Equation 26
\begin{dmath}
{MC}=\frac{{W}}{\left(1-{alpha}\right)\, {A}^{\frac{1}{1-{alpha}}}}\, {y}^{\frac{{alpha}}{1-{alpha}}}
\end{dmath}
% Equation 27
\begin{dmath}
{mu}=\frac{{pD}}{{MC}}
\end{dmath}
% Equation 28
\begin{dmath}
{e}={phi}\, {y}+{e}\, \left(1-{eta}\right)
\end{dmath}
% Equation 29
\begin{dmath}
\log\left({A}\right)=\left(1-{zetaA}\right)\, \log\left(({A})\right)+\log\left({A}\right)\, {zetaA}+{sA}
\end{dmath}
% Equation 30
\begin{dmath}
{PD}={pD}\, \left({e}\, {psi}\right)^{\frac{\left(-1\right)}{{sigma}-1}}
\end{dmath}
% Equation 31
\begin{dmath}
{Y}={A}\, \left({e}\, {psi}\right)^{\frac{1}{{sigma}-1}}\, {H}^{1-{alpha}}
\end{dmath}
% Equation 32
\begin{dmath}
{Y}={C}+{G}+\frac{{pD}\, {X}}{{P}}-\frac{{PF}}{{P}}\, \left({ACF}+{CF}+{GF}\right)
\end{dmath}
% Equation 33
\begin{dmath}
{PI}={P}\, {Y}-{H}\, {W}
\end{dmath}
% Equation 34
\begin{dmath}
{y}={Y}\, \left({e}\, {psi}\right)^{\frac{\left(-1\right)}{{sigma}-1}}
\end{dmath}
