% Equation 1
\begin{dmath}
\left({C}_{t}-\frac{{H}_{t}^{{omega}}}{{omega}}\right)^{\left(-{gamma}\right)}={lambda}_{t}\, {P}_{t}
\end{dmath}
% Equation 2
\begin{dmath}
\left({C}_{t}-\frac{{H}_{t}^{{omega}}}{{omega}}\right)^{\left(-{gamma}\right)}\, {H}_{t}^{{omega}-1}={lambda}_{t}\, {W}_{t}
\end{dmath}
% Equation 3
\begin{dmath}
{lambdaS}_{t}\, \left(1+{i}_{t}\right)={lambda}_{t}\, \left(1+{rho}\right)
\end{dmath}
% Equation 4
\begin{dmath}
{lambdaS}_{t}-{lambdaS}_{t-1}={sunspot}_{t}
\end{dmath}
% Equation 5
\begin{dmath}
{B}_{t}=\left(1+{i}_{t-1}\right)\, {B}_{t-1}+{H}_{t}\, {W}_{t}+{PI}_{t}-{T}_{t}-{C}_{t}\, {P}_{t}
\end{dmath}
% Equation 6
\begin{dmath}
{C}_{t}=\left(\left(1-{n}\right)^{\frac{1}{{s}}}\, {CD}_{t}^{\frac{{s}-1}{{s}}}+{n}^{\frac{1}{{s}}}\, {CF}_{t}^{\frac{{s}-1}{{s}}}\right)^{\frac{{s}}{{s}-1}}
\end{dmath}
% Equation 7
\begin{dmath}
{CD}_{t}={C}_{t}\, \left(1-{n}\right)\, \left(\frac{{PD}_{t}}{{P}_{t}}\right)^{\left(-{s}\right)}
\end{dmath}
% Equation 8
\begin{dmath}
{CF}_{t}={C}_{t}\, {n}\, \left(\frac{{PF}_{t}}{{P}_{t}}\right)^{\left(-{s}\right)}
\end{dmath}
% Equation 9
\begin{dmath}
{P}_{t}=\left(\left(1-{n}\right)\, {PD}_{t}^{1-{s}}+{n}\, {PF}_{t}^{1-{s}}\right)^{\frac{1}{1-{s}}}
\end{dmath}
% Equation 10
\begin{dmath}
{P}_{t}\, {G}_{t}={T}_{t}
\end{dmath}
% Equation 11
\begin{dmath}
\log\left({G}_{t}\right)=\left(1-{zetaG}\right)\, \log\left((\bar{G})\right)+{zetaG}\, \log\left({G}_{t-1}\right)+{sG}_{t}
\end{dmath}
% Equation 12
\begin{dmath}
{G}_{t}=\left(\left(1-{n}\right)^{\frac{1}{{s}}}\, {GD}_{t}^{\frac{{s}-1}{{s}}}+{n}^{\frac{1}{{s}}}\, {GF}_{t}^{\frac{{s}-1}{{s}}}\right)^{\frac{{s}}{{s}-1}}
\end{dmath}
% Equation 13
\begin{dmath}
{GD}_{t}=\left(1-{n}\right)\, \left(\frac{{PD}_{t}}{{P}_{t}}\right)^{\left(-{s}\right)}\, {G}_{t}
\end{dmath}
% Equation 14
\begin{dmath}
{GF}_{t}={n}\, \left(\frac{{PF}_{t}}{{P}_{t}}\right)^{\left(-{s}\right)}\, {G}_{t}
\end{dmath}
% Equation 15
\begin{dmath}
{i}_{t}=\left(1-{zetai}\right)\, (\bar{i})+{i}_{t-1}\, {zetai}+{kappa}\, \left(\exp\left(\frac{(\bar{B})}{(\bar{P})\, (\bar{Y})}-\frac{{B}_{t}}{{P}_{t}\, {Y}_{t}}\right)-1\right)+{si}_{t}
\end{dmath}
% Equation 16
\begin{dmath}
{AC}_{t}={Y}_{t}\, {P}_{t}\, \frac{{varphi}}{2}\, \left(\frac{{pD}_{t}}{{pD}_{t-1}}-1\right)^{2}
\end{dmath}
% Equation 17
\begin{dmath}
{ACD}_{t}=\left(1-{n}\right)\, \left(\frac{{PD}_{t}}{{P}_{t}}\right)^{\left(-{s}\right)}\, {AC}_{t}
\end{dmath}
% Equation 18
\begin{dmath}
{ACF}_{t}={n}\, \left(\frac{{PF}_{t}}{{P}_{t}}\right)^{\left(-{s}\right)}\, {AC}_{t}
\end{dmath}
% Equation 19
\begin{dmath}
{theta}_{t}\, {phi}={MC}_{t}-{pD}_{t}\, \frac{{sigma}-1}{{sigma}}-\frac{\frac{{pD}_{t}\, {Y}_{t}\, {P}_{t}\, \left(\frac{{pD}_{t}}{{pD}_{t-1}}-1\right)\, \frac{{varphi}}{{sigma}}}{{pD}_{t-1}}}{{y}_{t}}
\end{dmath}
% Equation 20
\begin{dmath}
\left(1+{rho}\right)\, {theta}_{t}=\frac{\frac{1}{{sigma}}\, {pDS}_{t}\, {yS}_{t}}{{e}_{t}}-\frac{\frac{{pDS}_{t}\, \frac{{varphi}}{{sigma}}\, \left(\frac{{pDS}_{t}}{{pD}_{t}}-1\right)}{{pD}_{t}}\, {PS}_{t}\, {YS}_{t}}{{e}_{t}}-\left(1-{eta}\right)\, {thetaS}_{t}
\end{dmath}
% Equation 21
\begin{dmath}
{pDS}_{t}-{pDS}_{t-1}={sunspot2}_{t}
\end{dmath}
% Equation 22
\begin{dmath}
{thetaS}_{t}-{thetaS}_{t-1}={sunspot3}_{t}
\end{dmath}
% Equation 23
\begin{dmath}
{yS}_{t}-{yS}_{t-1}={sunspot4}_{t}
\end{dmath}
% Equation 24
\begin{dmath}
{YS}_{t}-{YS}_{t-1}={sunspot5}_{t}
\end{dmath}
% Equation 25
\begin{dmath}
{PS}_{t}-{PS}_{t-1}={sunspot6}_{t}
\end{dmath}
% Equation 26
\begin{dmath}
{MC}_{t}=\frac{{W}_{t}}{\left(1-{alpha}\right)\, {A}_{t}^{\frac{1}{1-{alpha}}}}\, {y}_{t}^{\frac{{alpha}}{1-{alpha}}}
\end{dmath}
% Equation 27
\begin{dmath}
{mu}_{t}=\frac{{pD}_{t}}{{MC}_{t}}
\end{dmath}
% Equation 28
\begin{dmath}
{e}_{t}={phi}\, {y}_{t}+\left(1-{eta}\right)\, {e}_{t-1}
\end{dmath}
% Equation 29
\begin{dmath}
\log\left({A}_{t}\right)=\left(1-{zetaA}\right)\, \log\left((\bar{A})\right)+{zetaA}\, \log\left({A}_{t-1}\right)+{sA}_{t}
\end{dmath}
% Equation 30
\begin{dmath}
{PD}_{t}={pD}_{t}\, \left({e}_{t-1}\, {psi}\right)^{\frac{\left(-1\right)}{{sigma}-1}}
\end{dmath}
% Equation 31
\begin{dmath}
{Y}_{t}={A}_{t}\, \left({e}_{t-1}\, {psi}\right)^{\frac{1}{{sigma}-1}}\, {H}_{t}^{1-{alpha}}
\end{dmath}
% Equation 32
\begin{dmath}
{Y}_{t}={C}_{t}+{G}_{t}+\frac{{pD}_{t}\, {X}_{t}}{{P}_{t}}-\frac{{PF}_{t}}{{P}_{t}}\, \left({ACF}_{t}+{CF}_{t}+{GF}_{t}\right)
\end{dmath}
% Equation 33
\begin{dmath}
{PI}_{t}={P}_{t}\, {Y}_{t}-{H}_{t}\, {W}_{t}
\end{dmath}
% Equation 34
\begin{dmath}
{y}_{t}={Y}_{t}\, \left({e}_{t-1}\, {psi}\right)^{\frac{\left(-1\right)}{{sigma}-1}}
\end{dmath}
